online with alice-secrecy: small cleanup (#3)

examples/Online_with_secrecy/DY.OnlineS.Invariants.fst
@@ -33,14 +33,20 @@ open DY.OnlineS.Protocol
 %splice [ps_message_t_is_well_formed] (gen_is_well_formed_lemma (`message_t))
 
 
+
 // ignore this for now
 instance crypto_usages_p : crypto_usages = default_crypto_usages
 
 #push-options "--ifuel 2"
 let crypto_p : crypto_predicates = { 
   default_crypto_predicates with 
-  // we restrict when a message is allowed to be encrypted 
-  // with some secret key
+  (* we restrict when a message is allowed to be encrypted 
+     with some secret key
+
+     Or put differently:
+     What are the guarantees that an honest sender can provide
+     that are available at the receiver after decryption?
+  *)
   pkenc_pred = { 
     pred = (fun tr sk_usage msg ->
     exists prin. // the intended receiver of the message
@@ -53,6 +59,8 @@ let crypto_p : crypto_predicates = {
       (match parse message_t msg with
       | Some (Ping ping) ->
           (* a Ping message can only be encrypted if
+             (Or: if you decrypt a Ping from an honest party 
+             you get the guarantees that:)
              the contained nonce n_a
              is labeled for 
              * the name provided in the message (alice)
@@ -63,13 +71,7 @@ let crypto_p : crypto_predicates = {
           let n_a = ping.n_a in
           get_label tr n_a == nonce_label alice bob
       | Some (Ack ack) ->
-         (* an Ack message can only be encrypted if
-            the contained nonce n_a
-            is readable by the intended receiver (alice)
-         *)
-          let alice = prin in
-          let n_a = ack.n_a in
-          // get_label tr n_a `can_flow tr` principal_label alice
+         (* No conditions / guarantees needed for an Ack *)
           True
       | _ -> False // other messages can not be encrypted
       ))
@@ -122,14 +124,14 @@ let state_predicate_p: local_state_predicate state_t = {
     | SentAck ack -> (
         (* a SentAck state may only be stored if
            the stored nonce is readable by
-           * the storing principal (bob)
-           * the principal stored in the state 
-             (the intended receiver of the Ack: alice)
+           the storing principal (bob)
+
+           -- this is a condition that must always hold,
+           and is enforced by the `pred_knowable` Lemma.
         *)
         let bob = prin in
-        let alice = ack.alice in
         let n_a = ack.n_a in
-        is_knowable_by (nonce_label alice bob) tr n_a
+        is_knowable_by (principal_label bob) tr n_a
     )
     | ReceivedAck rack  -> (
         (* a ReceivedAck state may only be stored if
@@ -148,12 +150,17 @@ let state_predicate_p: local_state_predicate state_t = {
      if the state predicate holds on some trace tr1
      it also holds for any extension tr2 of tr2
   *)
-  pred_later = (fun tr1 tr2 prin sess_id st -> ());
+  pred_later = (fun tr1 tr2 prin sess_id st -> () );
   (* a lemma guaranteeing that
      the content of the state to be stored
      is readable by the storing principal
   *)
-  pred_knowable = (fun tr prin sess_id st -> ());
+  pred_knowable = (fun tr prin sess_id st -> 
+    match st with
+    | SentAck ack ->
+        parse_wf_lemma state_t (is_knowable_by (principal_label prin) tr) ack.n_a
+    | _ -> ()
+  );
 }
 #pop-options
 
