examples/Online_with_secrecy/DY.OnlineS.Secrecy.fst
@@ -31,9 +31,20 @@ val n_a_secrecy:
     attacker_knows tr n_a /\
     trace_invariant tr /\ (
       (exists sess_id. state_was_set tr alice sess_id (SentPing {bob; n_a})) \/
-      (exists sess_id. state_was_set tr bob sess_id (ReceivedAck {bob; n_a} ))
+      (exists sess_id. state_was_set tr alice sess_id (ReceivedAck {bob; n_a} ))
     )
   )
   (ensures is_corrupt tr (principal_label alice) \/ is_corrupt tr (principal_label bob))
+
+/// The proof idea is the following:
+/// For any nonce stored in one of Alice's states (SentPing or ReceivedAck)
+/// together with Bob,
+/// we get from the state predicate in the protocol invariants,
+/// that the nonce is labeled for exactly Alice and Bob.
+///
+/// This immediately means that one of Alice or Bob must be corrupted,
+/// if the attacker knows the nonce.
+/// The proof thus only consists of calling the main attacker lemma
+/// `attacker_only_knows_publishable_values`.
 let n_a_secrecy tr alice bob n_a =
   attacker_only_knows_publishable_values tr n_a
